fix FFI for ByteArray.slice

ffi.c
@@ -12,6 +12,7 @@ intern lean_sarray_object* mk_empty_byte_array(size_t len) {
     lean_set_st_header((lean_object*)o, LeanScalarArray, 1);
     o->m_size = len;
     o->m_capacity = len;
+    memset(o->m_data, 0, len);
     return o;
 }
 
@@ -38,15 +39,15 @@ extern l_res lean_uint64_to_byte_array(uint64_t n) {
     return mk_byte_array_from((void*)&n, 8);
 }
 
-extern l_res lean_byte_vector_to_uint16(l_arg a) {
+extern uint16_t lean_byte_vector_to_uint16(l_arg a) {
     return *((uint16_t*)lean_to_sarray(a)->m_data);
 }
 
-extern l_res lean_byte_vector_to_uint32(l_arg a) {
+extern uint32_t lean_byte_vector_to_uint32(l_arg a) {
     return *((uint32_t*)lean_to_sarray(a)->m_data);
 }
 
-extern l_res lean_byte_vector_to_uint64(l_arg a) {
+extern uint64_t lean_byte_vector_to_uint64(l_arg a) {
     return *((uint64_t*)lean_to_sarray(a)->m_data);
 }
 
@@ -73,20 +74,24 @@ extern uint8_t lean_byte_array_ord(l_arg a, l_arg b) {
     return 2;
 }
 
-extern l_res lean_byte_array_slice(l_arg a, size_t i, size_t n) {
+intern size_t nat_to_size_t(lean_obj_arg n) {
+    if (!lean_is_scalar(n))
+        lean_internal_panic("ByteArray.slice can't accept large parameters");
+    return lean_unbox(n);
+}
+
+extern l_res lean_byte_array_slice(l_arg a, lean_obj_arg oi, lean_obj_arg on) {
+    size_t i = nat_to_size_t(oi);
+    size_t n = nat_to_size_t(on);
     lean_sarray_object* oa = lean_to_sarray(a);
     size_t size = oa->m_size;
     lean_sarray_object* res = mk_empty_byte_array(n);
     if (i < size) {
         size_t copy_len;
         size_t would = i + n;
-        if (would < size) copy_len = would;
+        if (would < size) copy_len = would - i;
         else copy_len = size - i;
-        memcpy(
-            (void*)res->m_data,
-            (void*)oa->m_data + i * sizeof(uint8_t),
-            copy_len
-        );
+        memcpy(res->m_data, (oa->m_data + i * sizeof(uint8_t)), copy_len);
     }
     return (lean_object*)res;
 }
